theories/OGS/Subst.v
@@ -7,20 +7,6 @@ From OGS.Utils Require Import Ctx Psh Rel.
 
 Open Scope ctx_scope.
 
-Class baseT : Type :=
-  { typ : Type }.
-
-Class baseV `{baseT} : Type :=
-  { val : Famₛ typ }.
-
-Class baseC `{baseT} : Type :=
-  { conf : Fam typ }.
-
-Section withFam.
-  Context {bT : baseT}.
-  Context {bV : baseV}.
-  Context {bC : baseC}.
-
 (*|
 Substitution Monoid (Def. 4.9)
 ==============================
@@ -29,116 +15,128 @@ The specification of an evaluator will be separated in several steps. First we w
 i.e. objects that can be substituted for variables. We formalize well-typed well-scoped substitutions in the
 monoidal style of Fiore et al and Allais et al.
 |*)
-  Class subst_monoid : Type := {
-      v_var {Γ} : Γ =[val]> Γ ; (* Γ ∋ x -> val Γ x *)
-      v_sub {Γ Δ} : Γ =[val]> Δ -> val Γ ⇒ᵢ val Δ ;
-    }.
 
-  Notation "u ⊛ᵥ v" := (v_sub u _ v) (at level 30).
-  Notation "Γ ⇒ᵥ Δ" := (Γ =[val]> Δ) (at level 30).
+Class subst_monoid {T} (val : Famₛ T) : Type := {
+  v_var {Γ} : Γ =[val]> Γ ; (* Γ ∋ x -> val Γ x *)
+  v_sub {Γ Δ} : Γ =[val]> Δ -> val Γ ⇒ᵢ val Δ ;
+}.
+#[global] Notation "u ⊛ᵥ v" := (v_sub u _ v) (at level 30).
 
-  Context {VM : subst_monoid}.
-
-  Definition e_comp {Γ1 Γ2 Γ3} : Γ2 ⇒ᵥ Γ3 -> Γ1 ⇒ᵥ Γ2 -> Γ1 ⇒ᵥ Γ3
-    := fun u v => s_map (v_sub u) v.
-  Infix "⊛" := e_comp (at level 14).
+Definition e_comp {T val} {_ : @subst_monoid T val} {Γ1 Γ2 Γ3}
+  : Γ2 =[val]> Γ3 -> Γ1 =[val]> Γ2 -> Γ1 =[val]> Γ3
+  := fun u v => s_map (v_sub u) v.
+#[global] Infix "⊛" := e_comp (at level 14).
 
 (*|
-The laws for monoids and modules are pretty straitforward.
-A specificity is that assignments are represented
-by functions from variables to values, as such their well-behaved equality is
+The laws for monoids and modules are pretty straitforward. A specificity is that
+assignments are represented by functions from variables to values, as such their
+well-behaved equality is pointwise equality and we require substitution to respect it.
 |*)
-  Class subst_monoid_laws : Prop :=
-    {
-      v_sub_proper {Γ Δ} ::
-        Proper (ass_eq Γ Δ ==> forall_relation (fun i => eq ==> eq)) v_sub ;
-      v_sub_var {Γ1 Γ2} (p : Γ1 ⇒ᵥ Γ2) : p ⊛ v_var ≡ₐ p ;
-      v_var_sub {Γ1 Γ2} (p : Γ1 ⇒ᵥ Γ2) : v_var ⊛ p ≡ₐ p ;
-      v_sub_sub {Γ1 Γ2 Γ3 Γ4} (p : Γ3 ⇒ᵥ Γ4) (q : Γ2 ⇒ᵥ Γ3) (r : Γ1 ⇒ᵥ Γ2) :
-      p ⊛ (q ⊛ r) ≡ₐ (p ⊛ q) ⊛ r ;
-    } .
+
+Class subst_monoid_laws {T} (val : Famₛ T) {VM : subst_monoid val} : Prop := {
+  v_sub_proper {Γ Δ}
+    :: Proper (ass_eq Γ Δ ==> forall_relation (fun _ => eq ==> eq)) v_sub ;
+  v_sub_var {Γ1 Γ2} (p : Γ1 =[val]> Γ2)
+    : p ⊛ v_var ≡ₐ p ;
+  v_var_sub {Γ1 Γ2} (p : Γ1 =[val]> Γ2)
+    : v_var ⊛ p ≡ₐ p ;
+  v_sub_sub {Γ1 Γ2 Γ3 Γ4} (p : Γ3 =[val]> Γ4) (q : Γ2 =[val]> Γ3) (r : Γ1 =[val]> Γ2)
+   : p ⊛ (q ⊛ r) ≡ₐ (p ⊛ q) ⊛ r ;
+} .
 
 (*|
 Substitution Module (Def. 4.11)
-=================================
+===============================
 
-Next, we ask for a module over the monoid of values, to represent the configurations of the machine.
+Next, we ask for a module over the monoid of values, to represent the configurations
+of the machine.
 |*)
-  Class subst_module : Type := {
-      c_sub {Γ Δ} : Γ ⇒ᵥ Δ -> conf Γ -> conf Δ ;
-    }.
 
-  Notation "u ⊛ₜ c" := (c_sub u c) (at level 30).
+Class subst_module {T} (val : Famₛ T) (conf : Fam T) : Type := {
+  c_sub {Γ Δ} : Γ =[val]> Δ -> conf Γ -> conf Δ ;
+}.
 
-  Class subst_module_laws {CM : subst_module} : Prop := {
-    c_sub_proper {Γ Δ} :: Proper (ass_eq Γ Δ ==> eq ==> eq) c_sub ;
-    c_var_sub {Γ} (c : conf Γ) : v_var ⊛ₜ c = c ;
-    c_sub_sub {Γ1 Γ2 Γ3} (u : Γ2 ⇒ᵥ Γ3) (v : Γ1 ⇒ᵥ Γ2) {c}
-      : u ⊛ₜ (v ⊛ₜ c) = (u ⊛ v) ⊛ₜ c ;
-  } .
+#[global] Notation "u ⊛ₜ c" := (c_sub u c) (at level 30).
 
-(*|
-Additional assumptions on how variables behave.
-|*)
-  Definition is_var {Γ x} (v : val Γ x) : Type := { i : Γ ∋ x & v = v_var x i } .
-  Definition is_var_get {Γ x} {v : val Γ x} (p : is_var v) : Γ ∋ x := projT1 p .
-  Definition is_var_get_eq {Γ x} {v : val Γ x} (p : is_var v) : v = v_var x (is_var_get p) := projT2 p .
-
-  Context {CM : subst_module}.
+Class subst_module_laws {T} (val : Famₛ T) (conf : Fam T)
+      {VM : subst_monoid val} {CM : subst_module val conf} : Prop := {
+  c_sub_proper {Γ Δ} :: Proper (ass_eq Γ Δ ==> eq ==> eq) c_sub ;
+  c_var_sub {Γ} (c : conf Γ) : v_var ⊛ₜ c = c ;
+  c_sub_sub {Γ1 Γ2 Γ3} (u : Γ2 =[val]> Γ3) (v : Γ1 =[val]> Γ2) {c}
+    : u ⊛ₜ (v ⊛ₜ c) = (u ⊛ v) ⊛ₜ c ;
+} .
 
 (*|
 Derived notions: renamings.
 |*)
+
+Section renaming.
+  Context {T : Type} {val : Famₛ T} {conf : Fam T}.
+  Context {VM : subst_monoid val} {VML : subst_monoid_laws val}.
+  Context {CM : subst_module val conf} {CML : subst_module_laws val conf}.
+
   Definition v_ren {Γ Δ} : Γ ⊆ Δ -> val Γ ⇒ᵢ val Δ :=
     fun u => v_sub (v_var ⊛ᵣ u) .
-  Notation "r ᵣ⊛ᵥ v" := (v_ren r _ v) (at level 14).
 
-  Definition e_ren {Γ1 Γ2 Γ3} : Γ2 ⊆ Γ3 -> Γ1 ⇒ᵥ Γ2 -> Γ1 ⇒ᵥ Γ3
+  Definition e_ren {Γ1 Γ2 Γ3} : Γ2 ⊆ Γ3 -> Γ1 =[val]> Γ2 -> Γ1 =[val]> Γ3
     := fun u v => (v_var ⊛ᵣ u) ⊛ v.
-  Infix "ᵣ⊛" := e_ren (at level 14).
 
   Definition c_ren {Γ1 Γ2} : Γ1 ⊆ Γ2 -> conf Γ1 -> conf Γ2
     := fun u c => (v_var ⊛ᵣ u) ⊛ₜ c .
-  Infix "ᵣ⊛ₜ" := c_ren (at level 14).
+End renaming.
+#[global] Notation "r ᵣ⊛ᵥ v" := (v_ren r _ v) (at level 14).
+#[global] Infix "ᵣ⊛" := e_ren (at level 14).
+#[global] Infix "ᵣ⊛ₜ" := c_ren (at level 14).
 
-  Class var_assumptions : Type := {
-    v_var_inj {Γ x} (i j : Γ ∋ x) : v_var x i = v_var x j -> i = j ;
-    is_var_dec {Γ x} (v : val Γ x) : is_var v + (is_var v -> False) ;
-    is_var_ren {Γ1 Γ2 x} (v : val Γ1 x) (e : Γ1 ⊆ Γ2) : is_var (e ᵣ⊛ᵥ v) -> is_var v ;
-  }.
+(*|
+Additional assumptions on how variables behave. We basically ask that the identity
+assignment is injective, that being in its image is stable by renaming and that its
+image is decidable.
+|*)
 
-  Context {sVL: subst_monoid_laws}.
-  Context {sCL: subst_module_laws}.
-  Context {VA : var_assumptions} .
+Variant is_var {T} {val : Famₛ T} {VM : subst_monoid val} {Γ x} : val Γ x -> Type :=
+| IsVar (i : Γ ∋ x) : is_var (v_var x i)
+.
+Derive NoConfusion for is_var.
+
+Class var_assumptions {T} (val : Famₛ T) {VM : subst_monoid val} : Type := {
+  v_var_inj {Γ x} (i j : Γ ∋ x) : v_var x i = v_var x j -> i = j ;
+  is_var_dec {Γ x} (v : val Γ x) : is_var v + (is_var v -> False) ;
+  is_var_ren {Γ1 Γ2 x} (v : val Γ1 x) (e : Γ1 ⊆ Γ2) : is_var (e ᵣ⊛ᵥ v) -> is_var v ;
+}.
+
+Section variables.
+  Context {T : Type} (val : Famₛ T).
+  Context {VM : subst_monoid val} {VML : subst_monoid_laws val}.
+  Context {VA : var_assumptions val}.
 
   Lemma is_var_irr {Γ x} {v : val Γ x} (p q : is_var v) : p = q.
   Proof.
-    destruct p as [i1 e1], q as [i2 e2].
-    destruct (v_var_inj _ _ (eq_trans (eq_sym e1) e2)).
-    f_equal; apply YesUIP.
+    refine (match p as i in is_var v
+            return forall w (H : w = v) (q : is_var w), i = rew [is_var] H in q
+            with IsVar i => fun w H q => _
+            end v eq_refl q).
+    dependent elimination q.
+    pose proof (v_var_inj _ _ H) as H'.
+    now dependent elimination H'; dependent elimination H.
   Qed.
 
-  Definition ren_is_var {Γ1 Γ2 x} (v : val Γ1 x) (e : Γ1 ⊆ Γ2) : is_var v -> is_var (e ᵣ⊛ᵥ v).
+  Lemma ren_is_var {Γ1 Γ2 x} (v : val Γ1 x) (e : Γ1 ⊆ Γ2) : is_var v -> is_var (e ᵣ⊛ᵥ v).
   Proof.
-    intro p.
-    refine (e _ (is_var_get p) ,' _).
-    pose (i := is_var_get p); eassert (H : _) by exact (is_var_get_eq p); fold i in H |- *.
-    rewrite H; change (e ᵣ⊛ᵥ v_var x i) with ((e ᵣ⊛ v_var) x i).
-    unfold e_ren; rewrite v_sub_var; reflexivity.
-  Defined.
-
-  Variant is_var_ren_view {Γ1 Γ2 x} (v : val Γ1 x) (e : Γ1 ⊆ Γ2) : is_var (e ᵣ⊛ᵥ v) -> Type :=
-    | IsVarRen (p : is_var v) : is_var_ren_view v e (ren_is_var v e p)
-  .
-  Arguments IsVarRen {Γ1 Γ2 x v e}.
-
-  Lemma view_is_var_ren {Γ1 Γ2 x} (v : val Γ1 x) (e : Γ1 ⊆ Γ2) (p : is_var (e ᵣ⊛ᵥ v)) : is_var_ren_view v e p.
-    rewrite (is_var_irr p (ren_is_var v e (is_var_ren v e p))); econstructor.
+    intro p; dependent elimination p.
+    pose proof (v_sub_var (v_var ⊛ᵣ e) _ i) as H.
+    unfold v_ren, e_comp, s_map in *.
+    rewrite H; econstructor.
   Qed.
+End variables.
 
 (*|
 A couple derived properties on the constructed operations.
 |*)
+
+Section properties.
+  Context {T : Type} (val : Famₛ T).
+  Context {VM : subst_monoid val} {VML : subst_monoid_laws val}.
 
   #[global] Instance e_comp_proper {Γ1 Γ2 Γ3} :
     Proper (ass_eq Γ2 Γ3 ==> ass_eq Γ1 Γ2 ==> ass_eq Γ1 Γ3) e_comp.
@@ -154,40 +152,29 @@ A couple derived properties on the constructed operations.
     apply e_comp_proper; eauto; now rewrite H1.
   Qed.
 
-  Lemma e_comp_ren_r {Γ1 Γ2 Γ3 Γ4} (u : Γ3 ⇒ᵥ Γ4) (v : Γ2 ⇒ᵥ Γ3) (w : Γ1 ⊆ Γ2)
+  Lemma e_comp_ren_r {Γ1 Γ2 Γ3 Γ4} (u : Γ3 =[val]> Γ4) (v : Γ2 =[val]> Γ3) (w : Γ1 ⊆ Γ2)
     : u ⊛ (v ⊛ᵣ w) ≡ₐ (u ⊛ v) ⊛ᵣ w.
   Proof.
     reflexivity.
   Qed.
 
-  Lemma e_comp_ren_l {Γ1 Γ2 Γ3 Γ4} (u : Γ3 ⇒ᵥ Γ4) (v : Γ2 ⊆ Γ3) (w : Γ1 ⇒ᵥ Γ2)
+  Lemma e_comp_ren_l {Γ1 Γ2 Γ3 Γ4} (u : Γ3 =[val]> Γ4) (v : Γ2 ⊆ Γ3) (w : Γ1 =[val]> Γ2)
         : (u ⊛ᵣ v) ⊛ w ≡ₐ u ⊛ (v ᵣ⊛ w).
   Proof.
     unfold e_ren; now rewrite v_sub_sub, e_comp_ren_r, v_sub_var.
   Qed.
 
-  Lemma v_sub_comp {Γ1 Γ2 Γ3} (u : Γ2 ⇒ᵥ Γ3) (v : Γ1 ⇒ᵥ Γ2) {x} (w : val Γ1 x) :
+  Lemma v_sub_comp {Γ1 Γ2 Γ3} (u : Γ2 =[val]> Γ3) (v : Γ1 =[val]> Γ2) {x} (w : val Γ1 x) :
     u ⊛ᵥ (v ⊛ᵥ w) = (u ⊛ v) ⊛ᵥ w.
   Proof.
-    pose (w' := a_append a_empty w : (∅ ▶ x) ⇒ᵥ Γ1).
+    pose (w' := a_append a_empty w : (∅ ▶ x) =[val]> Γ1).
     change w with (w' _ Ctx.top).
     do 2 change (?u ⊛ᵥ ?v _ Ctx.top) with ((u ⊛ v) _ Ctx.top).
     apply v_sub_sub.
   Qed.
 
-  Lemma v_sub_id {Γ1 Γ2} (u : Γ1 ⇒ᵥ Γ2) {x} (i : Γ1 ∋ x) : u ⊛ᵥ (v_var x i) = u x i .
+  Lemma v_sub_id {Γ1 Γ2} (u : Γ1 =[val]> Γ2) {x} (i : Γ1 ∋ x) : u ⊛ᵥ (v_var x i) = u x i .
+  Proof.
     apply v_sub_var.
   Qed.
-
-End withFam.
-
-Arguments subst_monoid {_} _.
-Arguments subst_module {_} _ _.
-Notation "u ⊛ᵥ v" := (v_sub u _ v) (at level 30).
-Notation "Γ ⇒ᵥ Δ" := (Γ =[val]> Δ) (at level 30).
-Notation "u ⊛ₜ c" := (c_sub u c) (at level 30).
-Infix "⊛" := e_comp (at level 14).
-Notation "r ᵣ⊛ᵥ v" := (v_ren r _ v) (at level 14).
-Infix "ᵣ⊛" := e_ren (at level 14).
-Infix "ᵣ⊛ₜ" := c_ren (at level 14).
-
+End properties.
